coq/modular_proofs/EncodingBounds.v
@@ -1,0 +1,238 @@
+From Coq Require Import Arith.Arith Arith.PeanoNat Lists.List Lia.
+
+Lemma pow2_gt_succ : forall n, S n < Nat.pow 2 (S n).
+Proof.
+  intro n.
+  induction n as [|n IH]; simpl; [lia|].
+  assert (Hle : S (S n) <= 2 * S n) by lia.
+  assert (Hlt : 2 * S n < 2 * Nat.pow 2 (S n)).
+  { apply Nat.mul_lt_mono_pos_l; [lia|exact IH]. }
+  eapply Nat.le_lt_trans; [exact Hle|exact Hlt].
+Qed.
+
+Lemma pow_pos : forall a n, 1 <= a -> 0 < Nat.pow a n.
+Proof.
+  intros a n Ha.
+  induction n as [|n IH]; simpl; [lia|].
+  apply Nat.mul_pos_pos; [lia|exact IH].
+Qed.
+
+Section EncodingBounds.
+  Context (BASE SHIFT_LEN : nat).
+
+  Definition SHIFT_SMALL := Nat.pow BASE SHIFT_LEN.
+  Definition SHIFT_BIG := Nat.pow BASE (2 * SHIFT_LEN).
+
+  Context (BASE_ge_2 : 2 <= BASE).
+  Context (SHIFT_LEN_ge_1 : 1 <= SHIFT_LEN).
+
+  Lemma BASE_pos : 0 < BASE.
+  Proof. lia. Qed.
+
+  Lemma SHIFT_SMALL_pos : 0 < SHIFT_SMALL.
+  Proof.
+    unfold SHIFT_SMALL.
+    apply pow_pos; lia.
+  Qed.
+
+  Lemma SHIFT_SMALL_nonzero : SHIFT_SMALL <> 0.
+  Proof.
+    pose proof SHIFT_SMALL_pos as Hpos.
+    lia.
+  Qed.
+
+  Lemma shiftlen_lt_shiftsmall : SHIFT_LEN < SHIFT_SMALL.
+  Proof.
+    destruct SHIFT_LEN as [|len] eqn:Hlen; [lia|].
+    unfold SHIFT_SMALL.
+    simpl.
+    pose proof (pow2_gt_succ len) as Hpow.
+    assert (Hmono : Nat.pow 2 (S len) <= Nat.pow BASE (S len)).
+    { apply (Nat.pow_le_mono_l 2 BASE (S len)); lia. }
+    rewrite Hlen in *.
+    eapply Nat.lt_le_trans; [exact Hpow|exact Hmono].
+  Qed.
+
+  Lemma len_lt_SHIFT_SMALL : forall len, len <= SHIFT_LEN -> len < SHIFT_SMALL.
+  Proof.
+    intros len Hle.
+    eapply Nat.le_lt_trans; [exact Hle|apply shiftlen_lt_shiftsmall].
+  Qed.
+
+  Lemma SHIFT_BIG_as_product : SHIFT_BIG = SHIFT_SMALL * SHIFT_SMALL.
+  Proof.
+    unfold SHIFT_BIG, SHIFT_SMALL.
+    replace (2 * SHIFT_LEN) with (SHIFT_LEN + SHIFT_LEN) by lia.
+    rewrite Nat.pow_add_r.
+    reflexivity.
+  Qed.
+
+  Lemma SHIFT_SMALL_ge_succ_SHIFT_LEN : S SHIFT_LEN <= SHIFT_SMALL.
+  Proof.
+    assert (SHIFT_LEN < SHIFT_SMALL) by apply shiftlen_lt_shiftsmall.
+    lia.
+  Qed.
+
+  Lemma SHIFT_SMALL_le_SHIFT_BIG : SHIFT_SMALL <= SHIFT_BIG.
+  Proof.
+    rewrite SHIFT_BIG_as_product.
+    remember SHIFT_SMALL as s eqn:Hs.
+    destruct s as [|k].
+    { subst. pose proof SHIFT_SMALL_pos. lia. }
+    simpl.
+    rewrite Nat.mul_succ_r.
+    lia.
+  Qed.
+
+  Lemma SHIFT_LEN_lt_SHIFT_BIG : SHIFT_LEN < SHIFT_BIG.
+  Proof.
+    eapply Nat.lt_le_trans; [apply shiftlen_lt_shiftsmall|apply SHIFT_SMALL_le_SHIFT_BIG].
+  Qed.
+
+  Lemma le_SHIFT_LEN_lt_SHIFT_BIG :
+    forall x, x <= SHIFT_LEN -> x < SHIFT_BIG.
+  Proof.
+    intros x Hle.
+    apply Nat.lt_le_trans with (m := S SHIFT_LEN).
+    - lia.
+    - eapply Nat.le_trans; [apply SHIFT_SMALL_ge_succ_SHIFT_LEN|apply SHIFT_SMALL_le_SHIFT_BIG].
+  Qed.
+
+  Lemma lt_SHIFT_LEN_succ_lt_SHIFT_BIG :
+    forall x, x < SHIFT_LEN -> S x < SHIFT_BIG.
+  Proof.
+    intros x Hlt.
+    apply Nat.lt_le_trans with (m := S SHIFT_LEN).
+    - lia.
+    - eapply Nat.le_trans; [apply SHIFT_SMALL_ge_succ_SHIFT_LEN|apply SHIFT_SMALL_le_SHIFT_BIG].
+  Qed.
+
+  Lemma SHIFT_BIG_pos : 0 < SHIFT_BIG.
+  Proof.
+    rewrite SHIFT_BIG_as_product.
+    apply Nat.mul_pos_pos; apply SHIFT_SMALL_pos.
+  Qed.
+
+  Lemma SHIFT_BIG_nonzero : SHIFT_BIG <> 0.
+  Proof.
+    pose proof SHIFT_BIG_pos as Hpos.
+    lia.
+  Qed.
+
+  Lemma pack_lt_square : forall k a c, 0 < k -> a < k -> c < k -> a * k + c < k * k.
+  Proof.
+    intros k a c Hk Ha Hc.
+    apply Nat.lt_le_trans with (m := a * k + k).
+    - apply Nat.add_lt_mono_l; assumption.
+    - replace (a * k + k) with ((S a) * k) by (rewrite Nat.mul_succ_l; lia).
+      apply Nat.mul_le_mono_pos_r; lia.
+  Qed.
+
+  Lemma pair_fits_in_SHIFT_BIG :
+    forall len code,
+      len < SHIFT_SMALL ->
+      code < SHIFT_SMALL ->
+      len * SHIFT_SMALL + code < SHIFT_BIG.
+  Proof.
+    intros len code Hlen Hcode.
+    rewrite SHIFT_BIG_as_product.
+    apply pack_lt_square; try apply SHIFT_SMALL_pos; assumption.
+  Qed.
+
+  Section EncodeBounds.
+    Context (encode_list : list nat -> nat).
+    Context (digits_ok : list nat -> Prop).
+    Context (encode_list_upper : forall xs, digits_ok xs -> encode_list xs < Nat.pow BASE (length xs)).
+
+    Lemma encode_list_lt_SHIFT_SMALL :
+      forall xs,
+        digits_ok xs ->
+        length xs <= SHIFT_LEN ->
+        encode_list xs < SHIFT_SMALL.
+    Proof.
+      intros xs Hdig Hlen.
+      eapply Nat.lt_le_trans.
+      - apply encode_list_upper; assumption.
+      - unfold SHIFT_SMALL. apply Nat.pow_le_mono_r; lia.
+    Qed.
+
+    Lemma encode_list_len_code_small :
+      forall xs,
+        digits_ok xs ->
+        length xs <= SHIFT_LEN ->
+        length xs < SHIFT_SMALL /\ encode_list xs < SHIFT_SMALL.
+    Proof.
+      intros xs Hdig Hlen.
+      split.
+      - apply len_lt_SHIFT_SMALL; assumption.
+      - apply encode_list_lt_SHIFT_SMALL; assumption.
+    Qed.
+
+    Lemma encode_list_pack_lt_SHIFT_BIG :
+      forall xs,
+        digits_ok xs ->
+        length xs <= SHIFT_LEN ->
+        length xs * SHIFT_SMALL + encode_list xs < SHIFT_BIG.
+    Proof.
+      intros xs Hdig Hlen.
+      destruct (encode_list_len_code_small xs Hdig Hlen) as [Hlen_small Hcode_small].
+      apply pair_fits_in_SHIFT_BIG; assumption.
+    Qed.
+
+    Record encode_list_bounds (xs : list nat) := {
+      bounds_len_small : length xs < SHIFT_SMALL;
+      bounds_code_small : encode_list xs < SHIFT_SMALL;
+      bounds_packed_lt : length xs * SHIFT_SMALL + encode_list xs < SHIFT_BIG
+    }.
+
+    Lemma encode_list_bounds_of :
+      forall xs,
+        digits_ok xs ->
+        length xs <= SHIFT_LEN ->
+        encode_list_bounds xs.
+    Proof.
+      intros xs Hdig Hlen.
+      refine ({|
+        bounds_len_small := _;
+        bounds_code_small := _;
+        bounds_packed_lt := _
+      |}).
+      - apply len_lt_SHIFT_SMALL; assumption.
+      - apply encode_list_lt_SHIFT_SMALL; assumption.
+      - apply encode_list_pack_lt_SHIFT_BIG; assumption.
+    Qed.
+
+    Lemma encode_list_all_bounds :
+      forall xs,
+        digits_ok xs ->
+        length xs <= SHIFT_LEN ->
+        length xs < SHIFT_SMALL /\
+        encode_list xs < SHIFT_SMALL /\
+        length xs * SHIFT_SMALL + encode_list xs < SHIFT_BIG.
+    Proof.
+      intros xs Hdig Hlen.
+      destruct (encode_list_bounds_of xs Hdig Hlen) as [Hlen_small Hcode_small Hpacked_lt].
+      repeat split; assumption.
+    Qed.
+  End EncodeBounds.
+
+End EncodingBounds.
+
+Lemma div_mul_add_small :
+  forall k a c,
+    0 < k ->
+    c < k ->
+    ((a * k + c) / k = a) /\
+    ((a * k + c) mod k = c).
+Proof.
+  intros k a c Hk Hc.
+  split.
+  - assert (Hk' : k <> 0) by lia.
+    rewrite (Nat.div_add_l a k c) by exact Hk'.
+    rewrite (Nat.div_small c k) by exact Hc.
+    lia.
+  - rewrite Nat.add_comm.
+    rewrite Nat.Div0.mod_add.
+    rewrite Nat.mod_small by exact Hc.
+    reflexivity.
+Qed.
