coq/thielemachine/coqproofs/EncodingBridge.v
@@ -1,0 +1,29 @@
+From Coq Require Import List PeanoNat.
+Import ListNotations.
+
+From ThieleMachine.Modular_Proofs Require Import Encoding EncodingBounds.
+From ThieleUniversal Require Import TM.
+
+Definition tm_encode_config (conf : TMConfig) : nat :=
+  let '(q, tape, head) := conf in encode_config q tape head.
+
+Definition tm_decode_config (code : nat) : TMConfig :=
+  decode_config code.
+
+Definition tm_config_ok (conf : TMConfig) : Prop :=
+  let '(q, tape, head) := conf in
+  digits_ok tape /\ length tape <= SHIFT_LEN /\ head < SHIFT_LEN.
+
+Lemma tm_decode_encode_roundtrip :
+  forall conf,
+    tm_config_ok conf ->
+    tm_decode_config (tm_encode_config conf) = conf.
+Proof.
+  intros [[q tape] head] [Hdigs [Hlen Hhead]].
+  simpl in *.
+  pose proof (EncodingBounds.le_SHIFT_LEN_lt_SHIFT_BIG
+                Encoding.BASE Encoding.SHIFT_LEN
+                Encoding.BASE_ge_2 Encoding.SHIFT_LEN_ge_1
+                head (Nat.lt_le_incl _ _ Hhead)) as Hhead_big.
+  apply encode_decode_config; auto.
+Qed.
